LeanTab/Window.lean
@@ -5,10 +5,10 @@ set_option autoImplicit false
 namespace LeanTab
 
 def lag (xs : Array Cell) (n : Nat := 1) : Array Cell :=
-  (Array.mkArray (min n xs.size) Cell.na) ++ (xs.extract 0 (xs.size - n))
+  (Array.replicate (min n xs.size) Cell.na) ++ (xs.extract 0 (xs.size - n))
 
 def lead (xs : Array Cell) (n : Nat := 1) : Array Cell :=
-  (xs.extract n xs.size) ++ (Array.mkArray (min n xs.size) Cell.na)
+  (xs.extract n xs.size) ++ (Array.replicate (min n xs.size) Cell.na)
 
 def rowNumber (n : Nat) : Array Cell :=
   (Array.range n).map fun i => Cell.float (Float.ofNat (i + 1))
